Done
Co-authored-by: Sam Motto <sdmotto@users.noreply.github.com>
Co-authored-by: David Rhoades <David-Rhoadess@users.noreply.github.com>

code/UMap.dfy
@@ -16,45 +16,135 @@ import opened Option
 
 class UMap<T(!new,==)> {
 
+  var entrymap: Map<T>
+
   // this.entrySet() is the set of all the entries in the map 
   ghost function entrySet(): set<Entry<T>>
+  reads this
+  {
+    M.entries(this.entrymap)
+  }
 
   // this.keySet() is the set of all the keys in the map 
   ghost function keySet(): set<int>
+  reads this
+  requires isValid()
+  {
+    M.keys(this.entrymap)
+  }
 
   // this.valueSet() is the set of all the values in the map 
   ghost function valueSet(): set<T>
+  reads this
+  requires isValid()
+  {
+    M.values(this.entrymap)
+  }
 
   // A map m is valid iff it contains no repeated elements and
   // every key in m has exactly one associated value (no requires or ensures needed) 
-  ghost predicate isValid() 
+  ghost predicate isValid()
+  reads this
+  {
+    M.isValid(entrymap) &&
+    M.entries(entrymap) == entrySet()
+  }
 
-  // this.hasValue(k) is true iff key k as a value in the map
+  // this.hasValue(k) is true iff key k has a value in the map
   ghost predicate hasValue(k: int)
+  reads this
+  requires isValid()
+  ensures hasValue(k) <==> k in keySet()
+  {
+    None != M.get(this.entrymap, k)
+  }
 
   // this.isEmpty() is true iff the map contains no entries
   predicate isEmpty() 
+  reads this
+  requires isValid()
+  ensures isEmpty() <==> entrySet() == {}
+  {
+    M.isEmpty(entrymap)
+  }
 
   // constructor returns a (new) map with an empty set of entries.
   constructor ()
+  ensures isValid()
+  ensures entrySet() == {}
+  ensures keySet() == {}
+  ensures valueSet() == {}
+  {
+    entrymap := M.emptyMap<T>();
+  }
 
   // this.size() returns the number of entries in the map
   method size() returns (s: nat) 
+  requires isValid()
+  ensures s == |entrySet()|
+  {
+    s := M.size(entrymap);
+  }
 
   // this.get(k) returns the value associated to key k in the map, if any.
   // More precisely, it returns Some(v) if k has an associated value v,
   // and returns None otherwhise.
   method get(k: int) returns (vo: Option<T>)
+  requires isValid()
+  ensures vo == None <==> k !in keySet()
+  ensures forall v :: vo == Some(v) <==> (k, v) in entrySet()
+  {
+    vo := M.get(entrymap, k);
+  }
 
   // this.put(k, v) changes the map so that key k is associated with value v.
   // Then it returns the value previously associated to k in the map, if any.
   // More precisely, it returns Some(v) if k had an associated value v,
   // and returns None otherwhise.
   method put(k: int, v: T) returns (old_vo: Option<T>)
+  modifies this
+  requires isValid()
+  // We think these should hold but don't
 
-  // this.remove(k) removes from the map the entry eith key k, if any.
+  //ensures keySet() == old(keySet()) + {k}
+  //ensures valueSet == old(valueSet()) - {old_vo} + {v}
+  //ensures entrySet() == old(entrySet()) - {(k, old_vo)} + {(k, v)}
+  ensures isValid()
+  ensures k in keySet()
+  {
+    old_vo := M.get(entrymap, k);
+    entrymap := M.put(entrymap, k, v);
+  }
+
+  // this.remove(k) removes from the map the entry with key k, if any.
   // Then it returns the value previously associated to k in the map, if any.
   // More precisely, it returns Some(v) if k had an associated value v,
   // and returns None otherwhise.
   method remove(k: int) returns (vo: Option<T>)
+  modifies this
+  requires isValid()
+  ensures isValid()
+  ensures keySet() == old(keySet()) - {k}
+  {
+    vo := M.get(entrymap, k);
+    entrymap := M.remove(entrymap, k);
+  }
 }
+
+
+/*
+AI log (full project):
+Chatbot: GPT 5.1
+
+Prompt: How does Dafny "There exists" work
+Reflection: We used this to help write keys and values in part A. We knew the exists quanitifier existed in Dafny but could not 
+remember the syntax. GPTs response seemed reasonable and performed as expected in Dafny._
+
+Prompt: how can I access the value in a Dafny "Some" if I know it isn't none
+Reflection: This prompt was made in a moment of frustration at Dafny. GPT told us to use a .Value field but we did not end up needing this
+and moved on without using GPTs
+
+Prompt: do dafny constructors need a "ensures fresh" clause
+Reflection: GPT supported our assumption that we did not need to specify that constructors procude fresh values (becaue that is the entire
+and only point of a constructor). This was later confirmed in class. We used this when trying to debug the tests in part B.
+*/
